@prefix msm-nfp: <http://iserve.kmi.open.ac.uk/ns/msm-nfp#> .
@prefix owl: <http://www.w3.org/2002/07/owl#> .
@prefix rdf: <http://www.w3.org/1999/02/22-rdf-syntax-ns#> .
@prefix xml: <http://www.w3.org/XML/1998/namespace> .
@prefix xsd: <http://www.w3.org/2001/XMLSchema#> .
@prefix rdfs: <http://www.w3.org/2000/01/rdf-schema#> .
@prefix msm: <http://iserve.kmi.open.ac.uk/ns/msm#> .
@prefix dc: <http://purl.org/dc/terms/> .
@prefix sioc: <http://rdfs.org/sioc/ns#> .
@prefix foaf: <http://xmlns.com/foaf/0.1/> .
@prefix schema: <http://schema.org/> .

<http://iserve.kmi.open.ac.uk/ns/msm-nfp>
    a owl:Ontology ;
    rdfs:label "Minimal Service Model NFP ontology"@en ;
    dc:created "2015-10-01"^^xsd:date ;
	dc:issued "2015-10-01"^^xsd:date ;
    owl:versionInfo "0.3" ;
    dc:creator <http://kmi.open.ac.uk/> , <http://kmi.open.ac.uk/people/member/luca-panziera> ;
	dc:description "This ontology specifies non-functional properties that MSM services can assume"@en ;
    owl:imports <http://iserve.kmi.open.ac.uk/ns/msm> ,  <http://rdfs.org/sioc/ns#> , <http://xmlns.com/foaf/0.1/> .

msm-nfp:hasTotalMashups
    a rdf:Property ;
    rdfs:label "has applications"@en ;
    rdfs:comment "This property specifies the overall number of mashups in which the service is a component"@en ;
    rdfs:domain msm:Service ;
    rdfs:range xsd:int .

msm-nfp:hasRecentMashups
    a rdf:Property ;
    rdfs:label "has applications"@en ;
    rdfs:comment "This property specifies the number of mashups in which the service is a component in the last period"@en ;
    rdfs:domain msm:Service ;
    rdfs:range xsd:int .

msm-nfp:hasForum
    a rdf:Property ;
    rdfs:label "has forum"@en ;
    rdfs:domain msm:Service ;
    rdfs:range sioc:Forum .

msm-nfp:hasVitality
    a rdf:Property ;
    rdfs:label "has vitality"@en ;
    rdfs:comment "This property specifies the average of daily active users in the forum during the las period"@en ;
    rdfs:domain sioc:Forum ;
    rdfs:range xsd:double .

msm-nfp:hasPopularity
    a rdf:Property ;
    rdfs:label "has popularity"@en ;
    rdfs:comment "This property specifies the current index of popularity for an Organization or a Person"@en ;
    rdfs:domain schema:Organization, schema:Person ;
    rdfs:range xsd:double .

msm-nfp:hasTwitterAccount
    rdfs:subPropertyOf foaf:account ;
    rdfs:label "has Twitter account"@en ;
    rdfs:domain foaf:Agent ;
    rdfs:range msm-nfp:TwitterAccount .

msm-nfp:TwitterAccount
    rdfs:subClassOf foaf:OnlineAccount ;
    rdfs:label "Twitter account"@en ;
    rdfs:comment "Twitter account of a service"@en .

msm-nfp:hasDocumentation
    rdfs:subPropertyOf rdfs:seeAlso ;
    rdfs:label "has Documentation"@en ;
	rdfs:comment "This property specifies the documentation to consume the service. The documentation should be specified in natural language."@en ;
    rdfs:domain msm:Service ;
    rdfs:range rdfs:Resource .